@@ -1,6 +1,6 @@
 # Dataflow Analysis in Lean
 
-Subset of TIP as defined in _Static Program Analysis_.
+Subset of TIP as defined in _Static Program Analysis_. Approach influenced by _Principles of Program Analysis_.
 
 The goal is to develop complete, end-to-end proofs of dataflow soundness in Lean, establishing correctness of the procedure (fixpoint computation) as well as correctness wrt language semantics.
 
@@ -8,4 +8,8 @@ Progress:
 - [x] Formalized Kildall's worklist algorithm. 
   - [x] Proof of termination
   - [x] Proof of soundness
+- [x] Example of "mundane" correctness as described in PPA.
+  - [x] Constant propagation
+- [ ] Collection semantics proven by "mundane" correctness
+- [ ] Galois connections between collection semantics and further analyses.
 
